aarch64 ainvs: use machine_word for table indices
This replaces 'a word for indices with machine_word. Since we can't use
a specific word length for a generic table index (because different
tables can have different index types), we don't win much by using 'a
word, but we do lose something: we must instantiate 'a when we use the
term, which means we need to decide at that point which type of table
we are talking about. This forces early case distinctions in proofs.

Using machine_word allows us to delay committing to a particular table
type and instead write a generic condition on the width of the index.

We are using machine_word instead of nat or a different specific word
length, because the index into the table is a slice of either an
obj_ref (in ptes_of) or a vref (when we do page table walks), both of
which are compatible with machine_word.

Signed-off-by: Gerwin Klein <gerwin.klein@proofcraft.systems>

proof/invariant-abstract/AARCH64/ArchInvariants_AI.thy
@@ -294,9 +294,7 @@ primrec valid_pte :: "vm_level \<Rightarrow> pte \<Rightarrow> 'z::state_ext sta
      (\<lambda>s. normal_pt_at (ptrFromPAddr base) s \<and> 0 < level)"
 
 definition pt_range :: "pt \<Rightarrow> pte set" where
-  "pt_range pt \<equiv> case pt of VSRootPT vs \<Rightarrow> range vs | NormalPT pt \<Rightarrow> range pt"
-
-lemmas pt_range_simps[simp] = pt_range_def[split_simps pt.split]
+  "pt_range pt \<equiv> range (pt_apply pt)"
 
 fun valid_vspace_obj :: "vm_level \<Rightarrow> arch_kernel_obj \<Rightarrow> 'z::state_ext state \<Rightarrow> bool" where
   "valid_vspace_obj _ (ASIDPool pool) =
@@ -1087,19 +1085,14 @@ lemma pte_at_def2:
   "pte_at vsp p = (pt_at vsp (table_base vsp p) and K (is_aligned p pte_bits))"
   by (auto simp: pte_at_def level_pte_of_pt)
 
+lemmas pt_apply_def_simps[simp] = pt_apply_def[split_simps pt.split]
+
 lemma level_ptes_of_pts:
   "(level_pte_of vsp p (pts_of s) = Some pte) =
-   (\<exists>pt. pts_of s (table_base vsp p) = Some pt \<and> pt_pte pt p = pte \<and>
+   (\<exists>pt. pts_of s (table_base vsp p) = Some pt \<and> pt_apply pt (table_index vsp p) = pte \<and>
          is_aligned p pte_bits \<and> vsp = is_VSRootPT pt)"
   by (clarsimp simp: level_pte_of_def obj_at_def obind_def in_omonad opt_map_def
                split: option.splits)
-
-lemmas pt_pte_simps [simp] = pt_pte_def[split_simps pt.split]
-
-definition pt_apply :: "pt \<Rightarrow> machine_word \<Rightarrow> pte" where
-  "pt_apply pt idx \<equiv> case pt of NormalPT npt \<Rightarrow> npt (ucast idx) | VSRootPT vs \<Rightarrow> vs (ucast idx)"
-
-lemmas pt_apply_def_simps[simp] = pt_apply_def[split_simps pt.split]
 
 lemma ptes_of_Some:
   "(ptes_of s vsp p = Some pte) =
@@ -1167,6 +1160,29 @@ lemma in_user_frame_lift:
 lemma valid_vcpu_default[simp]:
   "valid_vcpu default_vcpu s"
   by (simp add: valid_vcpu_def default_vcpu_def)
+
+lemma pt_range_Normal[simp]:
+  "pt_range (NormalPT npt) = range npt"
+  unfolding pt_range_def
+  by (force intro: arg_cong[where f=npt] ucast_down_ucast_id[symmetric] simp: is_down)
+
+lemma pt_range_VSRoot[simp]:
+  "pt_range (VSRootPT vs) = range vs"
+  unfolding pt_range_def
+  by (force intro: arg_cong[where f=vs] ucast_down_ucast_id[symmetric] simp: is_down bit_simps)
+
+lemma pt_apply_pt_range[simp, intro!]:
+  "pt_apply pt idx \<in> pt_range pt"
+  by (auto simp: pt_range_def)
+
+lemma pt_apply_mask:
+  "pt_apply pt (idx && mask (ptTranslationBits (is_VSRootPT pt))) = pt_apply pt idx"
+  by (cases pt; clarsimp simp: bit_simps ucast_mask_drop)
+
+lemma pt_rangeD:
+  "pte \<in> pt_range pt \<Longrightarrow>
+   \<exists>idx. idx \<le> mask (ptTranslationBits (is_VSRootPT pt)) \<and> pt_apply pt idx = pte"
+  by (fastforce simp: pt_range_def intro!: word_and_le1 pt_apply_mask)
 
 lemma wellformed_arch_default[simp]:
   "arch_valid_obj (default_arch_object ao_type dev us) s"
@@ -1826,11 +1842,22 @@ lemma is_aligned_table_base_pte_bits[simp]:
   unfolding pte_bits_def
   by (simp add: bit_simps is_aligned_neg_mask)
 
-lemma pt_slot_offset_offset:
+lemma pt_index_bounded[simp, intro!]:
+  "pt_index level vref \<le> mask (ptTranslationBits (level = max_pt_level))"
+  by (simp add: pt_index_def word_and_le1)
+
+lemma table_index_plus:
+  "\<lbrakk> is_aligned pt_ptr (pt_bits vsp); i \<le> mask (ptTranslationBits vsp) \<rbrakk> \<Longrightarrow>
+   table_index vsp (pt_ptr + (i << pte_bits)) = i"
+  unfolding is_aligned_mask bit_simps
+  apply (cases "vsp \<and> config_ARM_PA_SIZE_BITS_40"; simp only:)
+   by (subst word_plus_and_or_coroll; word_bitwise; simp add: word_size)+
+
+lemma pt_slot_offset_offset[simp]:
   "is_aligned pt (pt_bits (level = max_pt_level)) \<Longrightarrow>
-   pt_slot_offset level pt vref && mask (pt_bits (level = max_pt_level)) >> pte_bits = pt_index level vref"
-  by (simp add: pt_slot_offset_def pt_index_def bit_simps mask_add_aligned and_mask_shiftr_comm
-                word_size and_mask2 mask_twice)
+   table_index (level = max_pt_level) (pt_slot_offset level pt vref) = pt_index level vref"
+  unfolding pt_slot_offset_def
+  by (simp add: table_index_plus)
 
 lemmas pt_slot_offset_minus_eq =
   pt_slot_offset_vref_for_level_eq[where level="level - 1" for level, simplified]
@@ -1847,52 +1874,6 @@ lemma table_base_plus:
   unfolding is_aligned_mask bit_simps
   apply (cases "vsp \<and> config_ARM_PA_SIZE_BITS_40"; simp only:)
    by (subst word_plus_and_or_coroll; word_bitwise; simp add: word_size)+
-
-
-lemma table_base_plus_ucast:
-  "is_aligned pt_ptr (pt_bits vsp) \<Longrightarrow>
-   table_base vsp (pt_ptr + (ucast (i::pt_index) << pte_bits)) = pt_ptr"
-  by (fastforce intro!: table_base_plus ucast_leq_mask simp: bit_simps)
-
-lemma table_index_plus:
-  "\<lbrakk> is_aligned pt_ptr (pt_bits vsp); i \<le> mask (ptTranslationBits vsp) \<rbrakk> \<Longrightarrow>
-   table_index vsp (pt_ptr + (i << pte_bits)) = ucast i"
-  unfolding is_aligned_mask bit_simps
-  apply (cases "vsp \<and> config_ARM_PA_SIZE_BITS_40"; simp only:)
-   by (subst word_plus_and_or_coroll; word_bitwise; simp add: word_size)+
-
-
-lemma table_index_plus_ucast:
-  "\<lbrakk> is_aligned pt_ptr (pt_bits vsp); LENGTH('a::len) = ptTranslationBits vsp \<rbrakk>  \<Longrightarrow>
-   table_index vsp (pt_ptr + (ucast (i::'a word) << pte_bits)) = i"
-  apply (drule table_index_plus[where i="ucast i" and 'a="'a"])
-   apply (rule ucast_leq_mask, simp add: bit_simps)
-  apply (simp add: is_down_def target_size_def source_size_def word_size ucast_down_ucast_id bit_simps)
-  done
-
-lemma table_index_plus_ucast_pt[simp]:
-  "is_aligned pt_ptr (pt_bits False) \<Longrightarrow>
-   table_index False (pt_ptr + (ucast (i::pt_index) << pte_bits)) = i"
-  by (rule table_index_plus_ucast; simp add: bit_simps)
-
-lemma table_index_plus_ucast_vs[simp]:
-  "is_aligned pt_ptr (pt_bits True) \<Longrightarrow>
-   table_index True (pt_ptr + (ucast (i::vs_index) << pte_bits)) = i"
-  by (rule table_index_plus_ucast; simp add: bit_simps)
-
-lemma table_index_offset_pt_bits_left_vs:
-  "\<lbrakk> is_aligned pt_ref (pt_bits True); lvl = max_pt_level \<rbrakk> \<Longrightarrow>
-   (table_index True (pt_slot_offset lvl pt_ref vref)::vs_index) =
-   ucast (vref >> pt_bits_left lvl)"
-  by (auto simp: table_index_plus_ucast pt_slot_offset_def pt_index_def vs_index_ptTranslationBits
-                 ucast_ucast_mask[where 'a=vs_index_len, simplified, symmetric])
-
-lemma table_index_offset_pt_bits_left_pt:
-  "\<lbrakk> is_aligned pt_ref (pt_bits False); lvl \<noteq> max_pt_level \<rbrakk> \<Longrightarrow>
-   (table_index False (pt_slot_offset lvl pt_ref vref)::pt_index) =
-   ucast (vref >> pt_bits_left lvl)"
-  by (simp add: table_index_plus_ucast pt_slot_offset_def pt_index_def
-                ptTranslationBits_def ucast_ucast_mask[where 'a=pt_index_len, simplified, symmetric])
 
 lemma vs_lookup_slot_level:
   "vs_lookup_slot bot_level asid vref s = Some (level, p) \<Longrightarrow>
@@ -2178,12 +2159,11 @@ lemma is_aligned_pt_slot_offset_pte:
   unfolding pt_slot_offset_def
   by (simp add: is_aligned_add bit_simps is_aligned_weaken is_aligned_shift)
 
-
 lemma pt_slot_offset_pt_range:
   "\<lbrakk> ptes_of s (level = max_pt_level) (pt_slot_offset level pt vref) = Some pte;
      pts_of s pt = Some ptable; is_aligned pt (pt_bits (level = max_pt_level)) \<rbrakk>
    \<Longrightarrow> pte \<in> pt_range ptable"
-  by (clarsimp simp: ptes_of_Some pt_apply_def split: pt.split)
+  by (clarsimp simp: ptes_of_Some)
 
 lemma valid_vspace_objs_strongD:
   "\<lbrakk> valid_vspace_objs s;
@@ -2432,41 +2412,25 @@ lemma vs_lookup_table_ap_step:
   apply (fastforce simp: vs_lookup_table_def vspace_for_pool_def entry_for_pool_def in_omonad)
   done
 
-locale_abbrev vref_for_index :: "'a::len word \<Rightarrow> vm_level \<Rightarrow> vspace_ref" where
-  "vref_for_index idx level \<equiv> ucast idx << pt_bits_left level"
+locale_abbrev vref_for_index :: "machine_word \<Rightarrow> vm_level \<Rightarrow> vspace_ref" where
+  "vref_for_index idx level \<equiv> idx << pt_bits_left level"
 
-locale_abbrev vref_for_level_idx :: "vspace_ref \<Rightarrow> 'a::len word \<Rightarrow> vm_level \<Rightarrow> vspace_ref" where
+locale_abbrev vref_for_level_idx :: "vspace_ref \<Rightarrow> machine_word \<Rightarrow> vm_level \<Rightarrow> vspace_ref" where
   "vref_for_level_idx vref idx level \<equiv> vref_for_level vref (level+1) || vref_for_index idx level"
 
+lemma pt_index_vref_for_level[simp]:
+  "\<lbrakk> level \<le> max_pt_level; idx \<le> mask (ptTranslationBits (level = max_pt_level)) \<rbrakk> \<Longrightarrow>
+  pt_index level (vref_for_level vref (level + 1) || vref_for_index idx level) = idx"
+  using pt_bits_left_bound[of "level"]
+  apply (simp add: pt_index_def vref_for_level_def pt_bits_left_bound_def)
+  apply word_eqI
+  by (auto simp: bit_simps pt_bits_left_def size_max_pt_level split: if_split_asm)
 
 lemma table_index_pt_slot_offset:
   "\<lbrakk> is_aligned p (pt_bits (level = max_pt_level)); level \<le> max_pt_level;
-     LENGTH('a) = ptTranslationBits (level = max_pt_level) \<rbrakk> \<Longrightarrow>
+     idx \<le> mask (ptTranslationBits (level = max_pt_level)) \<rbrakk> \<Longrightarrow>
    table_index (level = max_pt_level) (pt_slot_offset level p (vref_for_level_idx vref idx level)) = idx"
-  for idx::"'a::len word"
-  using pt_bits_left_bound[of "level"]
-  using pt_bits_left_bound[of "level+1"]
-  apply (simp add: pt_slot_offset_def pt_index_def vref_for_level_def pt_bits_left_bound_def)
-  apply (subst word_plus_and_or_coroll)
-   apply word_eqI
-   apply (clarsimp simp: bit_simps)
-  apply word_eqI
-  apply (clarsimp simp: bit_simps pt_bits_left_def split: if_split_asm)
-  done
-
-lemma table_index_pt_slot_offset_pt:
-  "\<lbrakk> is_aligned p (pt_bits False); level \<le> max_pt_level; level \<noteq> max_pt_level \<rbrakk> \<Longrightarrow>
-   ptable_index (pt_slot_offset level p (vref_for_level_idx vref idx level)) = idx"
-  for idx :: pt_index
-  using table_index_pt_slot_offset[where level=level and 'a=pt_index_len]
-  by (simp add: bit_simps)
-
-lemma table_index_pt_slot_offset_vs:
-  "\<lbrakk> is_aligned p (pt_bits True); level= max_pt_level \<rbrakk> \<Longrightarrow>
-   vsroot_index (pt_slot_offset level p (vref_for_level_idx vref idx level)) = idx"
-  for idx :: vs_index
-  using table_index_pt_slot_offset[where level=max_pt_level and 'a=vs_index_len]
-  by (simp add: bit_simps)
+  by simp
 
 lemma vs_lookup_vref_for_level_eq1:
   "vref_for_level vref' (bot_level+1) = vref_for_level vref (bot_level+1) \<Longrightarrow>
@@ -2479,10 +2443,9 @@ lemma vs_lookup_vref_for_level_eq1:
   done
 
 lemma vref_for_level_idx[simp]:
-  "\<lbrakk> level \<le> max_pt_level; LENGTH('a) = ptTranslationBits (level = max_pt_level) \<rbrakk> \<Longrightarrow>
+  "\<lbrakk> level \<le> max_pt_level; idx \<le> mask (ptTranslationBits (level = max_pt_level)) \<rbrakk> \<Longrightarrow>
    vref_for_level (vref_for_level_idx vref idx level) (level + 1) =
    vref_for_level vref (level + 1)"
-  for idx :: "'a::len word"
   apply (simp add: vref_for_level_def pt_bits_left_def)
   apply (rule conjI, clarsimp)
   apply (rule conjI; clarsimp; word_eqI_solve simp: bit_simps level_defs dest: bit_imp_possible_bit)
@@ -2505,17 +2468,16 @@ lemma vref_for_level_user_regionD:
 
 lemma vref_for_level_idx_canonical_user:
   "\<lbrakk> vref \<le> canonical_user; level \<le> max_pt_level;
-    LENGTH('a) = ptTranslationBits (level = max_pt_level);
-    level = max_pt_level \<longrightarrow> ucast idx \<notin> invalid_mapping_slots \<rbrakk> \<Longrightarrow>
+     idx \<le> mask (ptTranslationBits (level = max_pt_level));
+     level = max_pt_level \<longrightarrow> ucast idx \<notin> invalid_mapping_slots \<rbrakk> \<Longrightarrow>
    vref_for_level_idx vref idx level \<le> canonical_user"
-  for idx :: "'a::len word"
-  apply (simp add: canonical_user_def le_mask_high_bits ipa_size_def word_size split: if_split_asm)
+  apply (clarsimp simp: canonical_user_def le_mask_high_bits ipa_size_def word_size split: if_split_asm)
    apply (cases "level = max_pt_level")
-    apply (clarsimp simp: bit_simps pt_bits_left_def size_max_pt_level)
-    apply (drule bit_imp_possible_bit)
+    apply (simp add: bit_simps pt_bits_left_def size_max_pt_level asid_pool_level_eq word_size)
+    apply (frule bit_imp_possible_bit)
     apply simp
-   apply (clarsimp simp: bit_simps pt_bits_left_def size_max_pt_level asid_pool_level_eq)
-   apply (drule bit_imp_possible_bit)
+   apply (simp add: bit_simps pt_bits_left_def size_max_pt_level asid_pool_level_eq)
+   apply (frule bit_imp_possible_bit)
    apply simp
    apply (drule xt1(11), simp)
    apply (subst (asm) vm_level_size_less[symmetric])
@@ -2525,10 +2487,10 @@ lemma vref_for_level_idx_canonical_user:
    apply (frule bit_imp_possible_bit)
    apply simp
    apply (prop_tac "idx \<le> mask valid_vs_slot_bits")
-    apply (simp add: invalid_mapping_slots_def bit_simps le_mask_high_bits word_size)
+    apply (fastforce simp: invalid_mapping_slots_def bit_simps le_mask_high_bits word_size)
    apply (simp add: bit_simps le_mask_high_bits word_size)
-  apply (clarsimp simp: bit_simps pt_bits_left_def size_max_pt_level asid_pool_level_eq word_size)
-  apply (drule bit_imp_possible_bit)
+  apply (simp add: bit_simps pt_bits_left_def size_max_pt_level asid_pool_level_eq word_size)
+  apply (frule bit_imp_possible_bit)
   apply (drule xt1(11), simp)
   apply (subst (asm) vm_level_size_less[symmetric])
   apply (simp add: size_max_pt_level)
@@ -2541,28 +2503,9 @@ lemma vs_lookup_table_pt_step:
      valid_pt_range pt; pspace_distinct s \<rbrakk> \<Longrightarrow>
    \<exists>vref'. vs_lookup_target level asid vref' s = Some (level, p') \<and>
            vref' \<in> user_region"
-  apply (cases pt; clarsimp)
-   apply (rename_tac vs idx)
-   apply (rule_tac x="vref_for_level vref (level+1) ||
-                      (ucast (idx::vs_index) << pt_bits_left level)" in exI)
-   apply (simp add: vs_lookup_target_def vs_lookup_slot_def in_omonad)
-   apply (rule conjI)
-    apply (rule_tac x="pt_slot_offset level p (vref_for_level_idx vref idx level)" in exI)
-    apply (rule conjI, clarsimp)
-     apply (rule_tac x=level in exI)
-     apply (rule_tac x=p in exI)
-     apply clarsimp
-     apply (subst vs_lookup_vref_for_level_eq1)
-      prefer 2
-      apply assumption
-     apply (simp add: bit_simps)
-    apply (fastforce simp: ptes_of_Some in_omonad is_aligned_pt_slot_offset_pte
-                           table_index_pt_slot_offset_vs)
-   apply (prop_tac "idx \<notin> invalid_mapping_slots", clarsimp simp: valid_pt_range_def)
-   apply (simp add: user_region_def vref_for_level_idx_canonical_user bit_simps)
-  apply (rename_tac ptn idx)
-  apply (rule_tac x="vref_for_level vref (level+1) ||
-                     (ucast (idx::pt_index) << pt_bits_left level)" in exI)
+  apply (drule pt_rangeD, erule exE)
+  apply (rename_tac idx)
+  apply (rule_tac x="vref_for_level_idx vref idx level" in exI)
   apply (simp add: vs_lookup_target_def vs_lookup_slot_def in_omonad)
   apply (rule conjI)
    apply (rule_tac x="pt_slot_offset level p (vref_for_level_idx vref idx level)" in exI)
@@ -2575,10 +2518,12 @@ lemma vs_lookup_table_pt_step:
     apply (subst vs_lookup_vref_for_level_eq1)
      prefer 2
      apply assumption
-    apply (simp add: bit_simps)
-   apply (fastforce simp: ptes_of_Some in_omonad is_aligned_pt_slot_offset_pte
-                          table_index_pt_slot_offset_pt)
-  apply (simp add: user_region_def vref_for_level_idx_canonical_user bit_simps)
+    apply simp
+   apply (clarsimp simp: ptes_of_Some in_omonad is_aligned_pt_slot_offset_pte
+                         table_index_pt_slot_offset)
+  apply (prop_tac "is_VSRootPT pt \<longrightarrow> ucast idx \<notin> invalid_mapping_slots")
+   apply (cases pt; clarsimp simp: valid_pt_range_def)
+  apply (simp add: user_region_def vref_for_level_idx_canonical_user)
   done
 
 lemma pte_rights_PagePTE[simp]:
